libcrux-iot/sha3/proofs/libcrux-iot-sha3/lean/LibcruxIotSha3/Extraction/Specs.lean
@@ -78,31 +78,27 @@ def sha224_ema.pre
   else ok false
 
 /-- [libcrux_iot_sha3::sha224_ema::post]:
-    Source: 'sha3/src/lib.rs', lines 187:0-189:66 -/
+    Source: 'sha3/src/lib.rs', lines 187:0-188:66 -/
 @[reducible]
 def sha224_ema.post
   (digest : Slice Std.U8) (payload : Slice Std.U8)
   (digest_future : Slice Std.U8) :
   RustM Bool
   := do
-  let i ← core.slice.Slice.len digest_future
-  if i = SHA3_224_DIGEST_SIZE
-  then
-    let s ←
-      libcrux_secrets.SharedASlice.Insts.Libcrux_secretsTraitsDeclassifyRefSharedASlice.declassify_ref
-        libcrux_secrets.U8.Insts.Libcrux_secretsTraitsScalar digest_future
-    let s1 ←
-      libcrux_secrets.SharedASlice.Insts.Libcrux_secretsTraitsDeclassifyRefSharedASlice.declassify_ref
-        libcrux_secrets.U8.Insts.Libcrux_secretsTraitsScalar payload
-    let a ← hacspec_sha3.sha3.sha3_224 s1
-    let s2 ←
-      core.Array.Insts.CoreOpsIndexIndex.index
-        (core.Slice.Insts.CoreOpsIndexIndex
-        (core.ops.range.RangeFull.Insts.CoreSliceIndexSliceIndexSliceSlice
-        Std.U8)) a ()
-    core.Slice.Insts.CoreCmpPartialEqSlice.eq core.U8.Insts.CoreCmpPartialEqU8
-      s s2
-  else ok false
+  let s ←
+    libcrux_secrets.SharedASlice.Insts.Libcrux_secretsTraitsDeclassifyRefSharedASlice.declassify_ref
+      libcrux_secrets.U8.Insts.Libcrux_secretsTraitsScalar digest_future
+  let s1 ←
+    libcrux_secrets.SharedASlice.Insts.Libcrux_secretsTraitsDeclassifyRefSharedASlice.declassify_ref
+      libcrux_secrets.U8.Insts.Libcrux_secretsTraitsScalar payload
+  let a ← hacspec_sha3.sha3.sha3_224 s1
+  let s2 ←
+    core.Array.Insts.CoreOpsIndexIndex.index
+      (core.Slice.Insts.CoreOpsIndexIndex
+      (core.ops.range.RangeFull.Insts.CoreSliceIndexSliceIndexSliceSlice
+      Std.U8)) a ()
+  core.Slice.Insts.CoreCmpPartialEqSlice.eq core.U8.Insts.CoreCmpPartialEqU8 s
+    s2
 
 def sha224_ema.spec (digest : Slice Std.U8) (payload : Slice Std.U8) : Prop :=
   (sha224_ema.pre digest payload).holds →
@@ -112,7 +108,7 @@ def sha224_ema.spec (digest : Slice Std.U8) (payload : Slice Std.U8) : Prop :=
 
 
 /-- [libcrux_iot_sha3::sha256::pre]:
-    Source: 'sha3/src/lib.rs', lines 203:0-203:56 -/
+    Source: 'sha3/src/lib.rs', lines 202:0-202:56 -/
 @[reducible]
 def sha256.pre (payload : Slice Std.U8) : RustM Bool := do
   let i ← core.slice.Slice.len payload
@@ -127,7 +123,7 @@ def sha256.spec (payload : Slice Std.U8) : Prop :=
 
 
 /-- [libcrux_iot_sha3::sha256_ema::pre]:
-    Source: 'sha3/src/lib.rs', lines 216:0-216:96 -/
+    Source: 'sha3/src/lib.rs', lines 215:0-215:96 -/
 @[reducible]
 def sha256_ema.pre
   (digest : Slice Std.U8) (payload : Slice Std.U8) : RustM Bool := do
@@ -139,31 +135,27 @@ def sha256_ema.pre
   else ok false
 
 /-- [libcrux_iot_sha3::sha256_ema::post]:
-    Source: 'sha3/src/lib.rs', lines 217:0-219:66 -/
+    Source: 'sha3/src/lib.rs', lines 216:0-217:66 -/
 @[reducible]
 def sha256_ema.post
   (digest : Slice Std.U8) (payload : Slice Std.U8)
   (digest_future : Slice Std.U8) :
   RustM Bool
   := do
-  let i ← core.slice.Slice.len digest_future
-  if i = SHA3_256_DIGEST_SIZE
-  then
-    let s ←
-      libcrux_secrets.SharedASlice.Insts.Libcrux_secretsTraitsDeclassifyRefSharedASlice.declassify_ref
-        libcrux_secrets.U8.Insts.Libcrux_secretsTraitsScalar digest_future
-    let s1 ←
-      libcrux_secrets.SharedASlice.Insts.Libcrux_secretsTraitsDeclassifyRefSharedASlice.declassify_ref
-        libcrux_secrets.U8.Insts.Libcrux_secretsTraitsScalar payload
-    let a ← hacspec_sha3.sha3.sha3_256 s1
-    let s2 ←
-      core.Array.Insts.CoreOpsIndexIndex.index
-        (core.Slice.Insts.CoreOpsIndexIndex
-        (core.ops.range.RangeFull.Insts.CoreSliceIndexSliceIndexSliceSlice
-        Std.U8)) a ()
-    core.Slice.Insts.CoreCmpPartialEqSlice.eq core.U8.Insts.CoreCmpPartialEqU8
-      s s2
-  else ok false
+  let s ←
+    libcrux_secrets.SharedASlice.Insts.Libcrux_secretsTraitsDeclassifyRefSharedASlice.declassify_ref
+      libcrux_secrets.U8.Insts.Libcrux_secretsTraitsScalar digest_future
+  let s1 ←
+    libcrux_secrets.SharedASlice.Insts.Libcrux_secretsTraitsDeclassifyRefSharedASlice.declassify_ref
+      libcrux_secrets.U8.Insts.Libcrux_secretsTraitsScalar payload
+  let a ← hacspec_sha3.sha3.sha3_256 s1
+  let s2 ←
+    core.Array.Insts.CoreOpsIndexIndex.index
+      (core.Slice.Insts.CoreOpsIndexIndex
+      (core.ops.range.RangeFull.Insts.CoreSliceIndexSliceIndexSliceSlice
+      Std.U8)) a ()
+  core.Slice.Insts.CoreCmpPartialEqSlice.eq core.U8.Insts.CoreCmpPartialEqU8 s
+    s2
 
 def sha256_ema.spec (digest : Slice Std.U8) (payload : Slice Std.U8) : Prop :=
   (sha256_ema.pre digest payload).holds →
@@ -173,7 +165,7 @@ def sha256_ema.spec (digest : Slice Std.U8) (payload : Slice Std.U8) : Prop :=
 
 
 /-- [libcrux_iot_sha3::sha384::pre]:
-    Source: 'sha3/src/lib.rs', lines 233:0-233:56 -/
+    Source: 'sha3/src/lib.rs', lines 231:0-231:56 -/
 @[reducible]
 def sha384.pre (payload : Slice Std.U8) : RustM Bool := do
   let i ← core.slice.Slice.len payload
@@ -188,7 +180,7 @@ def sha384.spec (payload : Slice Std.U8) : Prop :=
 
 
 /-- [libcrux_iot_sha3::sha384_ema::pre]:
-    Source: 'sha3/src/lib.rs', lines 246:0-246:96 -/
+    Source: 'sha3/src/lib.rs', lines 244:0-244:96 -/
 @[reducible]
 def sha384_ema.pre
   (digest : Slice Std.U8) (payload : Slice Std.U8) : RustM Bool := do
@@ -200,31 +192,27 @@ def sha384_ema.pre
   else ok false
 
 /-- [libcrux_iot_sha3::sha384_ema::post]:
-    Source: 'sha3/src/lib.rs', lines 247:0-249:66 -/
+    Source: 'sha3/src/lib.rs', lines 245:0-246:66 -/
 @[reducible]
 def sha384_ema.post
   (digest : Slice Std.U8) (payload : Slice Std.U8)
   (digest_future : Slice Std.U8) :
   RustM Bool
   := do
-  let i ← core.slice.Slice.len digest_future
-  if i = SHA3_384_DIGEST_SIZE
-  then
-    let s ←
-      libcrux_secrets.SharedASlice.Insts.Libcrux_secretsTraitsDeclassifyRefSharedASlice.declassify_ref
-        libcrux_secrets.U8.Insts.Libcrux_secretsTraitsScalar digest_future
-    let s1 ←
-      libcrux_secrets.SharedASlice.Insts.Libcrux_secretsTraitsDeclassifyRefSharedASlice.declassify_ref
-        libcrux_secrets.U8.Insts.Libcrux_secretsTraitsScalar payload
-    let a ← hacspec_sha3.sha3.sha3_384 s1
-    let s2 ←
-      core.Array.Insts.CoreOpsIndexIndex.index
-        (core.Slice.Insts.CoreOpsIndexIndex
-        (core.ops.range.RangeFull.Insts.CoreSliceIndexSliceIndexSliceSlice
-        Std.U8)) a ()
-    core.Slice.Insts.CoreCmpPartialEqSlice.eq core.U8.Insts.CoreCmpPartialEqU8
-      s s2
-  else ok false
+  let s ←
+    libcrux_secrets.SharedASlice.Insts.Libcrux_secretsTraitsDeclassifyRefSharedASlice.declassify_ref
+      libcrux_secrets.U8.Insts.Libcrux_secretsTraitsScalar digest_future
+  let s1 ←
+    libcrux_secrets.SharedASlice.Insts.Libcrux_secretsTraitsDeclassifyRefSharedASlice.declassify_ref
+      libcrux_secrets.U8.Insts.Libcrux_secretsTraitsScalar payload
+  let a ← hacspec_sha3.sha3.sha3_384 s1
+  let s2 ←
+    core.Array.Insts.CoreOpsIndexIndex.index
+      (core.Slice.Insts.CoreOpsIndexIndex
+      (core.ops.range.RangeFull.Insts.CoreSliceIndexSliceIndexSliceSlice
+      Std.U8)) a ()
+  core.Slice.Insts.CoreCmpPartialEqSlice.eq core.U8.Insts.CoreCmpPartialEqU8 s
+    s2
 
 def sha384_ema.spec (digest : Slice Std.U8) (payload : Slice Std.U8) : Prop :=
   (sha384_ema.pre digest payload).holds →
@@ -234,7 +222,7 @@ def sha384_ema.spec (digest : Slice Std.U8) (payload : Slice Std.U8) : Prop :=
 
 
 /-- [libcrux_iot_sha3::sha512::pre]:
-    Source: 'sha3/src/lib.rs', lines 263:0-263:56 -/
+    Source: 'sha3/src/lib.rs', lines 260:0-260:56 -/
 @[reducible]
 def sha512.pre (payload : Slice Std.U8) : RustM Bool := do
   let i ← core.slice.Slice.len payload
@@ -249,7 +237,7 @@ def sha512.spec (payload : Slice Std.U8) : Prop :=
 
 
 /-- [libcrux_iot_sha3::sha512_ema::pre]:
-    Source: 'sha3/src/lib.rs', lines 276:0-276:96 -/
+    Source: 'sha3/src/lib.rs', lines 273:0-273:96 -/
 @[reducible]
 def sha512_ema.pre
   (digest : Slice Std.U8) (payload : Slice Std.U8) : RustM Bool := do
@@ -261,31 +249,27 @@ def sha512_ema.pre
   else ok false
 
 /-- [libcrux_iot_sha3::sha512_ema::post]:
-    Source: 'sha3/src/lib.rs', lines 277:0-279:66 -/
+    Source: 'sha3/src/lib.rs', lines 274:0-275:66 -/
 @[reducible]
 def sha512_ema.post
   (digest : Slice Std.U8) (payload : Slice Std.U8)
   (digest_future : Slice Std.U8) :
   RustM Bool
   := do
-  let i ← core.slice.Slice.len digest_future
-  if i = SHA3_512_DIGEST_SIZE
-  then
-    let s ←
-      libcrux_secrets.SharedASlice.Insts.Libcrux_secretsTraitsDeclassifyRefSharedASlice.declassify_ref
-        libcrux_secrets.U8.Insts.Libcrux_secretsTraitsScalar digest_future
-    let s1 ←
-      libcrux_secrets.SharedASlice.Insts.Libcrux_secretsTraitsDeclassifyRefSharedASlice.declassify_ref
-        libcrux_secrets.U8.Insts.Libcrux_secretsTraitsScalar payload
-    let a ← hacspec_sha3.sha3.sha3_512 s1
-    let s2 ←
-      core.Array.Insts.CoreOpsIndexIndex.index
-        (core.Slice.Insts.CoreOpsIndexIndex
-        (core.ops.range.RangeFull.Insts.CoreSliceIndexSliceIndexSliceSlice
-        Std.U8)) a ()
-    core.Slice.Insts.CoreCmpPartialEqSlice.eq core.U8.Insts.CoreCmpPartialEqU8
-      s s2
-  else ok false
+  let s ←
+    libcrux_secrets.SharedASlice.Insts.Libcrux_secretsTraitsDeclassifyRefSharedASlice.declassify_ref
+      libcrux_secrets.U8.Insts.Libcrux_secretsTraitsScalar digest_future
+  let s1 ←
+    libcrux_secrets.SharedASlice.Insts.Libcrux_secretsTraitsDeclassifyRefSharedASlice.declassify_ref
+      libcrux_secrets.U8.Insts.Libcrux_secretsTraitsScalar payload
+  let a ← hacspec_sha3.sha3.sha3_512 s1
+  let s2 ←
+    core.Array.Insts.CoreOpsIndexIndex.index
+      (core.Slice.Insts.CoreOpsIndexIndex
+      (core.ops.range.RangeFull.Insts.CoreSliceIndexSliceIndexSliceSlice
+      Std.U8)) a ()
+  core.Slice.Insts.CoreCmpPartialEqSlice.eq core.U8.Insts.CoreCmpPartialEqU8 s
+    s2
 
 def sha512_ema.spec (digest : Slice Std.U8) (payload : Slice Std.U8) : Prop :=
   (sha512_ema.pre digest payload).holds →
@@ -295,14 +279,14 @@ def sha512_ema.spec (digest : Slice Std.U8) (payload : Slice Std.U8) : Prop :=
 
 
 /-- [libcrux_iot_sha3::shake128::pre]:
-    Source: 'sha3/src/lib.rs', lines 293:0-293:48 -/
+    Source: 'sha3/src/lib.rs', lines 289:0-289:48 -/
 @[reducible]
 def shake128.pre (BYTES : Std.Usize) (data : Slice Std.U8) : RustM Bool := do
   let i ← lift (UScalar.cast .Usize core.num.U32.MAX)
   ok (BYTES <= i)
 
 /-- [libcrux_iot_sha3::shake128::post]:
-    Source: 'sha3/src/lib.rs', lines 294:0-295:63 -/
+    Source: 'sha3/src/lib.rs', lines 290:0-291:63 -/
 @[reducible]
 def shake128.post
   {BYTES : Std.Usize} (data : Slice Std.U8) (out : Array Std.U8 BYTES) :
@@ -324,7 +308,7 @@ def shake128.spec (BYTES : Std.Usize) (data : Slice Std.U8) : Prop :=
 
 
 /-- [libcrux_iot_sha3::shake128_ema::pre]:
-    Source: 'sha3/src/lib.rs', lines 309:0-309:52 -/
+    Source: 'sha3/src/lib.rs', lines 305:0-305:52 -/
 @[reducible]
 def shake128_ema.pre
   (out : Slice Std.U8) (data : Slice Std.U8) : RustM Bool := do
@@ -340,14 +324,14 @@ def shake128_ema.spec (out : Slice Std.U8) (data : Slice Std.U8) : Prop :=
 
 
 /-- [libcrux_iot_sha3::shake256::pre]:
-    Source: 'sha3/src/lib.rs', lines 318:0-318:48 -/
+    Source: 'sha3/src/lib.rs', lines 314:0-314:48 -/
 @[reducible]
 def shake256.pre (BYTES : Std.Usize) (data : Slice Std.U8) : RustM Bool := do
   let i ← lift (UScalar.cast .Usize core.num.U32.MAX)
   ok (BYTES <= i)
 
 /-- [libcrux_iot_sha3::shake256::post]:
-    Source: 'sha3/src/lib.rs', lines 319:0-320:63 -/
+    Source: 'sha3/src/lib.rs', lines 315:0-316:63 -/
 @[reducible]
 def shake256.post
   {BYTES : Std.Usize} (data : Slice Std.U8) (out : Array Std.U8 BYTES) :
@@ -369,7 +353,7 @@ def shake256.spec (BYTES : Std.Usize) (data : Slice Std.U8) : Prop :=
 
 
 /-- [libcrux_iot_sha3::shake256_ema::pre]:
-    Source: 'sha3/src/lib.rs', lines 334:0-334:52 -/
+    Source: 'sha3/src/lib.rs', lines 330:0-330:52 -/
 @[reducible]
 def shake256_ema.pre
   (out : Slice Std.U8) (data : Slice Std.U8) : RustM Bool := do
@@ -385,7 +369,7 @@ def shake256_ema.spec (out : Slice Std.U8) (data : Slice Std.U8) : Prop :=
 
 
 /-- [libcrux_iot_sha3::keccakx1::pre]:
-    Source: 'sha3/src/lib.rs', lines 546:0-548:2 -/
+    Source: 'sha3/src/lib.rs', lines 542:0-544:2 -/
 @[reducible]
 def keccakx1.pre
   (RATE : Std.Usize) (DELIM : Std.U8) (data : Slice Std.U8)
@@ -1280,7 +1264,7 @@ def state.KeccakState.set_lane.spec (self : state.KeccakState) (i : Std.Usize)
 
 
 /-- [libcrux_iot_sha3::incremental::{impl libcrux_iot_sha3::incremental::Xof<168usize> for libcrux_iot_sha3::incremental::Shake128Xof}::absorb::pre]:
-    Source: 'sha3/src/lib.rs', lines 427:8-430:10 -/
+    Source: 'sha3/src/lib.rs', lines 423:8-426:10 -/
 @[reducible]
 def incremental.XofShake128Xof168.absorb.pre
   (self_ : incremental.Shake128Xof) (input : Slice Std.U8) : RustM Bool := do
@@ -1305,7 +1289,7 @@ def incremental.Shake128Xof.Insts.Libcrux_iot_sha3IncrementalXof168.absorb.spec
 
 
 /-- [libcrux_iot_sha3::incremental::{impl libcrux_iot_sha3::incremental::Xof<168usize> for libcrux_iot_sha3::incremental::Shake128Xof}::absorb_final::pre]:
-    Source: 'sha3/src/lib.rs', lines 435:8-438:10 -/
+    Source: 'sha3/src/lib.rs', lines 431:8-434:10 -/
 @[reducible]
 def incremental.XofShake128Xof168.absorb_final.pre
   (self_ : incremental.Shake128Xof) (input : Slice Std.U8) : RustM Bool := do
@@ -1331,7 +1315,7 @@ def
 
 
 /-- [libcrux_iot_sha3::incremental::{impl libcrux_iot_sha3::incremental::Xof<136usize> for libcrux_iot_sha3::incremental::Shake256Xof}::absorb::pre]:
-    Source: 'sha3/src/lib.rs', lines 456:8-459:10 -/
+    Source: 'sha3/src/lib.rs', lines 452:8-455:10 -/
 @[reducible]
 def incremental.XofShake256Xof136.absorb.pre
   (self_ : incremental.Shake256Xof) (input : Slice Std.U8) : RustM Bool := do
@@ -1356,7 +1340,7 @@ def incremental.Shake256Xof.Insts.Libcrux_iot_sha3IncrementalXof136.absorb.spec
 
 
 /-- [libcrux_iot_sha3::incremental::{impl libcrux_iot_sha3::incremental::Xof<136usize> for libcrux_iot_sha3::incremental::Shake256Xof}::absorb_final::pre]:
-    Source: 'sha3/src/lib.rs', lines 464:8-467:10 -/
+    Source: 'sha3/src/lib.rs', lines 460:8-463:10 -/
 @[reducible]
 def incremental.XofShake256Xof136.absorb_final.pre
   (self_ : incremental.Shake256Xof) (input : Slice Std.U8) : RustM Bool := do
